theories/Definitions.v
@@ -1,0 +1,69 @@
+From Coq Require Import
+     Classes.CRelationClasses.
+From Equations.Type Require
+     Classes.
+Require Import Relation_Definitions String.
+From Em Require Import
+     Context Environment Prelude.
+Import ctx.
+Import ctx.notations.
+
+Notation World := (Ctx nat).
+Definition TYPE : Type := World -> Type.
+Definition Valid (A : TYPE) : Type :=
+  forall w, A w.
+Definition Impl (A B : TYPE) : TYPE :=
+  fun w => A w -> B w.
+Definition Forall {I : Type} (A : I -> TYPE) : TYPE :=
+  fun w => forall i : I, A i w.
+
+(* pure  :: a -> f a *)
+(* apply :: f (a -> b) -> f a -> f b *)
+
+
+(* η   : Valid (Impl Unit (f unit)) *)
+(* <*> : f a -> f b -> f (a * b) *)
+
+Declare Scope indexed_scope.
+Bind Scope indexed_scope with TYPE.
+
+Notation "⊢ A" := (Valid A) (at level 100).
+Notation "A -> B" := (Impl A B) : indexed_scope.
+
+Definition Unit : TYPE := fun _ => unit.
+Definition Option (A : TYPE) : TYPE := fun w => option (A w).
+Definition List (A : TYPE) : TYPE := fun w => list (A w).
+Definition Prod (A B : TYPE) : TYPE := fun w => prod (A w) (B w).
+Definition Sum (A B : TYPE) : TYPE := fun w => sum (A w) (B w).
+
+Definition BoxR (R : Relation.relation World) (A : TYPE) : TYPE :=
+  fun w0 => forall w1, R w0 w1 -> A w1.
+
+(* Notation "◻A" := BoxR A *)
+
+Definition DiamondR (R : Relation.relation World) (A : TYPE) : TYPE :=
+  fun w0 => {w1 & R w0 w1 * A w1}%type.
+
+Notation "[< R >] A" := (BoxR R A) (at level 9, format "[< R >] A", right associativity).
+
+Module acc.
+
+  Inductive Accessibility (Σ₁ : World) : TYPE :=
+    | refl    : Accessibility Σ₁ Σ₁
+    | fresh α : forall Σ₂, Accessibility (Σ₁ ▻ α) Σ₂ ->
+                              Accessibility Σ₁ Σ₂.
+
+End acc.
+
+(* Everything is now qualified, except the stuff in paren on the line below *)
+Export acc (Accessibility).
+
+(* □ A *)
+Definition Box (A : TYPE) : TYPE :=
+  fun w => forall w', Accessibility w w' -> A w'.
+
+(* TODO: switch to superscript *)
+(* \^s \^+ *)
+
+Notation "◻₊ A" := (Box A) (at level 9, format "◻₊ A", right associativity)
+    : indexed_scope.
